Custom `simplify_map_eq` with default registers

theories/opsem/machine_base.v
@@ -1614,9 +1614,9 @@ Qed.
 
 Definition lookup_reg (r : RegName) (regs : Reg) : option Word :=
   w ← (regs !! r);
-  Some (if (bool_decide (r = cnull)) then (WInt 0) else w).
+  Some (if (decide (r = cnull)) then (WInt 0) else w).
 Definition insert_reg (r : RegName) (w : Word) (regs : Reg) : Reg :=
-  let w' := if (bool_decide (r = cnull)) then (WInt 0) else w in
+  let w' := if (decide (r = cnull)) then (WInt 0) else w in
   <[r:=w']>regs.
 
 Notation "m !!ᵣ i" := (lookup_reg i m) (at level 20) : stdpp_scope.
@@ -1638,8 +1638,7 @@ Proof.
   intros Hr.
   rewrite /lookup_reg.
   destruct (regs !! r) ; cbn ; last done.
-  destruct (bool_decide (r = cnull)) eqn:Hdec; cbn in *; try done.
-  apply bool_decide_eq_true in Hdec; done.
+  destruct (decide (r = cnull)) eqn:Hdec; cbn in *; try done.
 Qed.
 
 Lemma elem_of_dom_reg (regs : Reg) (r : RegName) :
@@ -1665,36 +1664,18 @@ Proof.
   done.
 Qed.
 
-Lemma lookup_reg_insert_ne r1 r2 w regs :
-  r1 ≠ r2 -> (<[r1:=w]> regs) !!ᵣ r2 = regs !!ᵣ r2.
-Proof.
-  intros Hneq.
-  rewrite /lookup_reg.
-  rewrite lookup_insert_ne; auto.
-Qed.
-
-Lemma lookup_reg_insert r w regs :
-  (<[r:=w]> regs) !!ᵣ r = (if (decide (r = cnull)) then Some (WInt 0) else Some w).
-Proof.
-  destruct (decide (r = cnull)); simplify_eq; rewrite /lookup_reg; simplify_map_eq.
-  + rewrite bool_decide_eq_true_2; auto.
-  + rewrite bool_decide_eq_false_2; auto.
-Qed.
-
 Lemma insert_reg_insert r w1 w2 regs :
   <[ r := w1 ]ᵣ> (<[ r := w2 ]> regs) = <[ r := w1 ]ᵣ> regs.
 Proof.
-  destruct (decide (r = cnull)); simplify_eq; rewrite /insert_reg; simplify_map_eq.
-  + rewrite bool_decide_eq_true_2; auto; by rewrite insert_insert.
-  + rewrite bool_decide_eq_false_2; auto; by rewrite insert_insert.
+  destruct (decide (r = cnull)) eqn:Hdec; simplify_eq; rewrite /insert_reg
+  ; rewrite Hdec; by rewrite insert_insert.
 Qed.
 
 Lemma insert_insert_reg r w1 w2 regs :
   <[ r := w1 ]> (<[ r := w2 ]ᵣ> regs) = <[ r := w1 ]> regs.
 Proof.
-  destruct (decide (r = cnull)); simplify_eq; rewrite /insert_reg; simplify_map_eq.
-  + rewrite bool_decide_eq_true_2; auto; by rewrite insert_insert.
-  + rewrite bool_decide_eq_false_2; auto; by rewrite insert_insert.
+  destruct (decide (r = cnull)) eqn:Hdec; simplify_eq; rewrite /insert_reg
+  ; rewrite Hdec; by rewrite insert_insert.
 Qed.
 
 Lemma insert_reg_insert_commute r1 r2 w1 w2 regs :
@@ -1703,3 +1684,244 @@ Lemma insert_reg_insert_commute r1 r2 w1 w2 regs :
 Proof.
   intros Hneq. rewrite insert_commute; auto.
 Qed.
+
+Lemma lookup_reg_singleton_None r1 r2 w :
+  ({[r1 := w]} : Reg) !!ᵣ r2 = None ↔ r1 ≠ r2.
+Proof.
+  rewrite /lookup_reg.
+  split; intros H.
+  - intros ->; rewrite lookup_singleton in H; done.
+  - eapply lookup_singleton_None in H; rewrite H; auto.
+    Unshelve. 1: exact Word. 1: auto.
+Qed.
+
+Lemma lookup_reg_empty r :
+  (∅ : Reg) !!ᵣ r = None.
+Proof.
+  rewrite /lookup_reg.
+  rewrite lookup_empty; done.
+Qed.
+
+Lemma lookup_insert_reg regs r w :
+  <[r:=w]ᵣ> regs !! r = Some (if (decide (r = cnull)) then WInt 0 else w).
+Proof.
+  destruct (decide (r = cnull)) eqn:Hdec; simplify_eq; rewrite /insert_reg
+  ; rewrite Hdec; by rewrite lookup_insert.
+Qed.
+Lemma lookup_insert_reg_ne regs r1 r2 w :
+  r1 ≠ r2 -> <[r1:=w]ᵣ> regs !! r2 = regs !! r2.
+Proof.
+  intros Hneq.
+  rewrite /lookup_reg.
+  rewrite lookup_insert_ne; auto.
+Qed.
+
+Lemma lookup_reg_insert regs r w :
+  (<[r:=w]> regs) !!ᵣ r = Some (if (decide (r = cnull)) then WInt 0 else w).
+Proof.
+  destruct (decide (r = cnull)) eqn:Hdec; simplify_eq; rewrite /lookup_reg
+  ; rewrite Hdec; by rewrite lookup_insert.
+Qed.
+
+Lemma lookup_reg_insert_ne regs r1 r2 w :
+  r1 ≠ r2 -> (<[r1:=w]> regs) !!ᵣ r2 = regs !!ᵣ r2.
+Proof.
+  intros Hneq.
+  rewrite /lookup_reg.
+  rewrite lookup_insert_ne; auto.
+Qed.
+
+Lemma lookup_reg_insert_reg regs r w :
+  <[r:=w]ᵣ> regs !!ᵣ r = Some (if (decide (r = cnull)) then WInt 0 else w).
+Proof.
+  destruct (decide (r = cnull)) eqn:Hdec; simplify_eq; rewrite /lookup_reg /insert_reg
+  ; rewrite Hdec; by rewrite lookup_insert.
+Qed.
+
+Lemma lookup_reg_insert_reg_ne regs r1 r2 w :
+  r1 ≠ r2 -> <[r1:=w]ᵣ> regs !!ᵣ r2 = regs !!ᵣ r2.
+Proof.
+  intros Hneq.
+  rewrite /lookup_reg.
+  rewrite lookup_insert_ne; auto.
+Qed.
+
+Lemma lookup_reg_delete regs r :
+  delete r regs !!ᵣ r = None.
+Proof.
+  rewrite /lookup_reg.
+  by rewrite lookup_delete.
+Qed.
+Lemma lookup_reg_delete_ne regs r1 r2 :
+  r1 ≠ r2 -> delete r1 regs !!ᵣ r2 = regs !!ᵣ r2.
+Proof.
+  intros Hneq.
+  rewrite /lookup_reg.
+  rewrite lookup_delete_ne; auto.
+Qed.
+Lemma lookup_reg_singleton r w :
+  ({[r := w]} : Reg) !!ᵣ r = Some (if (decide (r = cnull)) then WInt 0 else w).
+Proof.
+  rewrite /lookup_reg.
+  rewrite lookup_singleton; auto; cbn.
+Qed.
+Lemma lookup_reg_singleton_ne r1 r2 w :
+  r1 ≠ r2 -> ({[r1 := w]} : Reg) !!ᵣ r2 = None.
+Proof.
+  intros Hneq.
+  rewrite /lookup_reg.
+  rewrite lookup_singleton_ne; auto.
+Qed.
+
+Lemma lookup_reg_singleton_Some r1 r2 w1 w2 :
+  ({[r1 := w1]} : Reg) !!ᵣ r2 = Some w2 ↔ r1 = r2 ∧ (if (decide (r2 = cnull)) then WInt 0 else w1)
+  = w2.
+Proof.
+  split; rewrite /lookup_reg; intros H.
+  - destruct ({[r1 := w1]} !! r2) eqn:Hr2; cbn in *; last done.
+    apply lookup_singleton_Some in Hr2 as [-> ->].
+    split; simplify_eq; done.
+  - destruct H as [-> <-].
+    by rewrite lookup_singleton; cbn.
+Qed.
+
+Lemma lookup_reg_weaken_inv (regs1 regs2 : Reg) (r : RegName) (w1 w2 : Word) :
+  regs1 !!ᵣ r = Some w1 → regs1 ⊆ regs2 → regs2 !!ᵣ r = Some w2 -> w1 = w2.
+Proof.
+  intros Hr1 Hincl Hr2.
+  rewrite /lookup_reg in Hr1.
+  rewrite /lookup_reg in Hr2.
+  destruct (regs1 !! r) eqn:Hr; cbn in *; last done.
+  simplify_eq.
+  eapply lookup_weaken in Hr; eauto.
+  rewrite Hr in Hr2; cbn in *.
+  simplify_eq.
+  done.
+Qed.
+
+Lemma insert_reg_not_cnull (regs : Reg) (r : RegName) (w : Word) :
+  r ≠ cnull -> <[r := w]ᵣ> regs = <[r := w]> regs.
+Proof.
+  intros Hr.
+  rewrite /insert_reg.
+  destruct (decide (r = cnull)); done.
+Qed.
+
+Tactic Notation "simpl_map_regs" "by" tactic3(tac) :=
+  repeat (match goal with
+          | H : context [ _ !!ᵣ ?r ] |- _ =>
+              rewrite lookup_reg_not_cnull in H; [|by tac]
+          | H : context [ <[ _ := _]ᵣ> _ ] |- _ =>
+              rewrite insert_reg_not_cnull in H; [|by tac]
+          | |- context [ _ !!ᵣ ?r ] =>
+              rewrite lookup_reg_not_cnull; [|by tac]
+          | |- context [ <[ _ := _]ᵣ> _ ] =>
+              rewrite insert_reg_not_cnull; [|by tac]
+          end).
+
+Tactic Notation "simpl_map" "by" tactic3(tac) :=
+  repeat
+  match goal with
+  | H : context[ ∅ !! _ ] |- _ => rewrite lookup_empty in H
+  | H : context[ ∅ !!ᵣ _ ] |- _ => rewrite lookup_reg_empty in H
+  | H : context[ (<[_:=_]>_) !! _ ] |- _ =>
+    rewrite lookup_insert in H || (rewrite lookup_insert_ne in H; [| by tac])
+  | H : context[ (<[_:=_]ᵣ>_) !! _ ] |- _ =>
+    rewrite lookup_insert_reg in H || (rewrite lookup_insert_reg_ne in H; [| by tac])
+  | H : context[ (<[_:=_]>_) !!ᵣ _ ] |- _ =>
+    rewrite lookup_reg_insert in H || (rewrite lookup_reg_insert_ne in H; [| by tac])
+  | H : context[ (<[_:=_]ᵣ>_) !!ᵣ _ ] |- _ =>
+    rewrite lookup_reg_insert_reg in H || (rewrite lookup_reg_insert_reg_ne in H; [| by tac])
+  | H : context[ (alter _ _ _) !! _] |- _ =>
+    rewrite lookup_alter in H || (rewrite lookup_alter_ne in H; [| by tac])
+  | H : context[ (delete _ _) !! _] |- _ =>
+    rewrite lookup_delete in H || (rewrite lookup_delete_ne in H; [| by tac])
+  | H : context[ (delete _ _) !!ᵣ _] |- _ =>
+    rewrite lookup_reg_delete in H || (rewrite lookup_reg_delete_ne in H; [| by tac])
+  | H : context[ {[ _ := _ ]} !! _ ] |- _ =>
+    rewrite lookup_singleton in H || (rewrite lookup_singleton_ne in H; [| by tac])
+  | H : context[ {[ _ := _ ]} !!ᵣ _ ] |- _ =>
+    rewrite lookup_reg_singleton in H || (rewrite lookup_reg_singleton_ne in H; [| by tac])
+  | H : context[ (_ <$> _) !! _ ] |- _ => rewrite lookup_fmap in H
+  | H : context[ (omap _ _) !! _ ] |- _ => rewrite lookup_omap in H
+  | H : context[ lookup (A:=?A) ?i (?m1 ∪ ?m2) ] |- _ =>
+    let x := fresh in evar (x:A);
+    let x' := eval unfold x in x in clear x;
+    let E := fresh in
+    assert ((m1 ∪ m2) !! i = Some x') as E by (clear H; by tac);
+    rewrite E in H; clear E
+  | |- context[ ∅ !! _ ] => rewrite lookup_empty
+  | |- context[ ∅ !!ᵣ _ ] => rewrite lookup_reg_empty
+  | |- context[ (<[_:=_]>_) !! _ ] =>
+    rewrite lookup_insert || (rewrite lookup_insert_ne; [| by tac])
+  | |- context[ (<[_:=_]ᵣ>_) !!ᵣ _ ] =>
+    rewrite lookup_reg_insert_reg || (rewrite lookup_reg_insert_reg_ne; [| by tac])
+  | |- context[ (<[_:=_]ᵣ>_) !! _ ] =>
+    rewrite lookup_insert_reg || (rewrite lookup_insert_reg_ne; [| by tac])
+  | |- context[ (<[_:=_]>_) !!ᵣ _ ] =>
+    rewrite lookup_reg_insert || (rewrite lookup_reg_insert_ne; [| by tac])
+  | |- context[ (alter _ _ _) !! _ ] =>
+    rewrite lookup_alter || (rewrite lookup_alter_ne; [| by tac])
+  | |- context[ (delete _ _) !! _ ] =>
+    rewrite lookup_delete || (rewrite lookup_delete_ne; [| by tac])
+  | |- context[ (delete _ _) !!ᵣ _ ] =>
+    rewrite lookup_reg_delete || (rewrite lookup_reg_delete_ne; [| by tac])
+  | |- context[ {[ _ := _ ]} !! _ ] =>
+    rewrite lookup_singleton || (rewrite lookup_singleton_ne; [| by tac])
+  | |- context[ {[ _ := _ ]} !!ᵣ _ ] =>
+    rewrite lookup_reg_singleton || (rewrite lookup_reg_singleton_ne; [| by tac])
+  | |- context[ (_ <$> _) !! _ ] => rewrite lookup_fmap
+  | |- context[ (omap _ _) !! _ ] => rewrite lookup_omap
+  | |- context [ lookup (A:=?A) ?i ?m ] =>
+    let x := fresh in evar (x:A);
+    let x' := eval unfold x in x in clear x;
+    let E := fresh in
+    assert (m !! i = Some x') as E by tac;
+    rewrite E; clear E
+  end.
+
+
+Tactic Notation "simplify_map_eq" "by" tactic3(tac) :=
+  decompose_map_disjoint;
+  repeat match goal with
+  | _ => progress simpl_map_regs by tac
+  | _ => progress simpl_map by tac
+  | _ => progress simplify_eq/=
+  | _ => progress simpl_option by tac
+  | H : {[ _ := _ ]} !! _ = None |- _ => rewrite lookup_singleton_None in H
+  | H : {[ _ := _ ]} !!ᵣ _ = None |- _ => rewrite lookup_reg_singleton_None in H
+  | H : {[ _ := _ ]} !! _ = Some _ |- _ =>
+    rewrite lookup_singleton_Some in H; destruct H
+  | H : {[ _ := _ ]} !!ᵣ _ = Some _ |- _ =>
+    rewrite lookup_reg_singleton_Some in H; destruct H
+  | H1 : ?m1 !! ?i = Some ?x, H2 : ?m2 !! ?i = Some ?y |- _ =>
+    let H3 := fresh in
+    opose proof (lookup_weaken_inv m1 m2 i x y) as H3; [done|by tac|done|];
+    clear H2; symmetry in H3
+  | H1 : ?m1 !!ᵣ ?i = Some ?x, H2 : ?m2 !!ᵣ ?i = Some ?y |- _ =>
+    let H3 := fresh in
+    opose proof (lookup_reg_weaken_inv m1 m2 i x y) as H3; [done|by tac|done|];
+    clear H2; symmetry in H3
+    (*----- *)
+  | H1 : ?m1 !! ?i = Some ?x, H2 : ?m2 !! ?i = None |- _ =>
+    let H3 := fresh in
+    apply (lookup_weaken _ m2) in H1; [congruence|by tac]
+  | H1 : ?m1 !!ᵣ ?i = Some ?x, H2 : ?m2 !!ᵣ ?i = None |- _ =>
+    let H3 := fresh in
+    apply (lookup_reg_weaken _ m2) in H1; [congruence|by tac]
+  | H : ?m ∪ _ = ?m ∪ _ |- _ =>
+    apply map_union_cancel_l in H; [|by tac|by tac]
+  | H : _ ∪ ?m = _ ∪ ?m |- _ =>
+    apply map_union_cancel_r in H; [|by tac|by tac]
+  | H : {[?i := ?x]} = ∅ |- _ => by destruct (map_non_empty_singleton i x)
+  | H : ∅ = {[?i := ?x]} |- _ => by destruct (map_non_empty_singleton i x)
+  | H : ?m !! ?i = Some _, H2 : ?m !! ?j = None |- _ =>
+     unless (i ≠ j) by done;
+     assert (i ≠ j) by (by intros ?; simplify_eq)
+  end.
+Tactic Notation "simplify_map_eq" "/=" "by" tactic3(tac) :=
+  repeat (progress csimpl in * || simplify_map_eq by tac).
+Tactic Notation "simplify_map_eq" :=
+  simplify_map_eq by eauto with simpl_map map_disjoint.
+Tactic Notation "simplify_map_eq" "/=" :=
+  simplify_map_eq/= by eauto with simpl_map map_disjoint.
